ocamllibs/src/consynth/Findloops.ml
@@ -3,7 +3,7 @@ open Format
 open LoopsHelper
 open Utils
 open Utils.ListTools
-open PpHelper
+open Utils.PpTools
 open VariableAnalysis
 
 module E = Errormsg
