ocamllibs/test/to_solve/anbn_with_count.c
@@ -1,0 +1,13 @@
+_Bool example_0star1star_cnt (_Bool *ar, int n) {
+  _Bool an = 1;
+  _Bool bn = 1;
+  int cnt = 0;
+
+  for(int i = 0; i < n; i++) {
+    an = (ar [i]) && an;
+    bn = ((! ar [i]) || an) && bn;
+    cnt = cnt + (ar[i]? 1: -1);
+  }
+
+  return cnt;
+}
