synth_times.py
@@ -1,0 +1,15 @@
+import matplotlib.pyplot as plt
+import matplotlib.cbook as cbook
+import numpy as np
+
+data = np.genfromtxt('synth_times.csv', delimiter=',', skip_header=0,
+                     skip_footer=0, names=['example_name', 'synth_time'])
+fig = plt.figure()
+ax1 = fig.add_subplot(111)
+
+ax1.set_title("Synthesis times")
+ax1.set_xlabel('Example name')
+ax1.set_ylabel('Synthesis time')
+
+
+ax1.plot(data['example_name'], data['synth_time'], color='r', label='Synthesis times')
