ocamllibs/dafny_examples/Example_line_sight.dfy
@@ -5,15 +5,18 @@ function DfMax(x: int, y: int): int { if x > y then x else y}
 
 function Aux_1(a : seq<int>): int
 requires |a| >= 1
-{ if |a| == 1 then  a[0] else  a[|a|-1] 
+{
+  if |a| == 1 then a[0] else a[|a|-1]
 }
 
 function Amax(a : seq<int>): int
-{ if a == [] then  0 else  DfMax(Amax(a[..|a|-1]), a[|a|-1]) 
+{
+  if a == [] then 0 else DfMax(Amax(a[..|a|-1]), a[|a|-1])
 }
 
 function Visible(a : seq<int>): bool
-{ if a == [] then  true else  (Amax(a[..|a|-1]) <= a[|a|-1]) 
+{
+  if a == [] then true else (Amax(a[..|a|-1]) <= a[|a|-1])
 }
 
 function Aux_1Join(leftAux_1 : int, rightAux_1 : int): int
@@ -32,12 +35,19 @@ function VisibleJoin(leftAux_1 : int, leftAmax : int, rightAux_1 : int, rightAma
 }
 
 
+lemma BaseCaseAux_1(a : seq<int>, R_a : seq<int>)
+  requires |a| >= 1 && |R_a| >= 1
+  ensures Aux_1(a + [R_a[0]]) == Aux_1Join(Aux_1(a), Aux_1([R_a[0]]))
+  {}
+
 lemma HomAux_1(a : seq<int>, R_a : seq<int>)
+  requires |a| >= 1 && |R_a| >= 1
   ensures Aux_1(a + R_a) == Aux_1Join(Aux_1(a), Aux_1(R_a))
   {
     if |R_a| == 1 
     {
     assert(a + R_a == a + [R_a[0]]);
+    BaseCaseAux_1(a, R_a);
     
      } else {
     calc{
@@ -48,17 +58,12 @@ lemma HomAux_1(a : seq<int>, R_a : seq<int>)
   } // End else.
 } // End lemma.
 
-lemma BaseCaseAmax(a : seq<int>)
-  ensures Amax(a) == AmaxJoin(Amax(a), Amax([]))
-  {}
-
 lemma HomAmax(a : seq<int>, R_a : seq<int>)
   ensures Amax(a + R_a) == AmaxJoin(Amax(a), Amax(R_a))
   {
     if R_a == [] 
     {
     assert(a + [] == a);
-    BaseCaseAmax(a);
     
      } else {
     calc{
@@ -69,12 +74,19 @@ lemma HomAmax(a : seq<int>, R_a : seq<int>)
   } // End else.
 } // End lemma.
 
+lemma BaseCaseVisible(a : seq<int>, R_a : seq<int>)
+  requires |a| >= 1 && |R_a| >= 1
+  ensures Visible(a + [R_a[0]]) == VisibleJoin(Aux_1(a), Amax(a), Aux_1([R_a[0]]), Amax([R_a[0]]))
+  {}
+
 lemma HomVisible(a : seq<int>, R_a : seq<int>)
+  requires |a| >= 1 && |R_a| >= 1
   ensures Visible(a + R_a) == VisibleJoin(Aux_1(a), Amax(a), Aux_1(R_a), Amax(R_a))
   {
-    if R_a == [] 
+    if |R_a| == 1 
     {
-    assert(a + [] == a);
+    assert(a + R_a == a + [R_a[0]]);
+    BaseCaseVisible(a, R_a);
     
      } else {
     calc{
