ocamllibs/dafny_examples/Example_0after1.dfy
@@ -2,19 +2,21 @@ function DfLength(s: seq<int>): int
 {if s == [] then 0 else DfLength(s[..|s|-1]) + 1}
 
 function Aux_2(a : seq<bool>): bool
-{ if a == [] then  false else  ((! a[|a|-1]) || Aux_2(a[..|a|-1])) 
+{
+  if a == [] then false else ((! a[|a|-1]) || Aux_2(a[..|a|-1]))
 }
 
 function Seen1(a : seq<bool>): bool
-{ if a == [] then  false else  (Seen1(a[..|a|-1]) || a[|a|-1]) 
+{
+  if a == [] then false else (Seen1(a[..|a|-1]) || a[|a|-1])
 }
 
 function Res(a : seq<bool>): bool
-{ if a == [] then
+{
+  if a == [] then
     false
-   else 
-   (((! a[|a|-1]) && Seen1(a[..|a|-1])) || Res(a[..|a|-1]))
-   
+    else
+    (((! a[|a|-1]) && Seen1(a[..|a|-1])) || Res(a[..|a|-1]))
 }
 
 function Aux_2Join(leftAux_2 : bool, rightAux_2 : bool): bool
@@ -33,17 +35,12 @@ function ResJoin(leftAux_2 : bool, leftRes : bool, leftSeen1 : bool, rightAux_2 
 }
 
 
-lemma BaseCaseAux_2(a : seq<bool>)
-  ensures Aux_2(a) == Aux_2Join(Aux_2(a), Aux_2([]))
-  {}
-
 lemma HomAux_2(a : seq<bool>, R_a : seq<bool>)
   ensures Aux_2(a + R_a) == Aux_2Join(Aux_2(a), Aux_2(R_a))
   {
     if R_a == [] 
     {
     assert(a + [] == a);
-    BaseCaseAux_2(a);
     
      } else {
     calc{
@@ -54,17 +51,12 @@ lemma HomAux_2(a : seq<bool>, R_a : seq<bool>)
   } // End else.
 } // End lemma.
 
-lemma BaseCaseSeen1(a : seq<bool>)
-  ensures Seen1(a) == Seen1Join(Res(a), Seen1(a), Res([]), Seen1([]))
-  {}
-
 lemma HomSeen1(a : seq<bool>, R_a : seq<bool>)
   ensures Seen1(a + R_a) == Seen1Join(Res(a), Seen1(a), Res(R_a), Seen1(R_a))
   {
     if R_a == [] 
     {
     assert(a + [] == a);
-    BaseCaseSeen1(a);
     
      } else {
     calc{
@@ -78,17 +70,12 @@ lemma HomSeen1(a : seq<bool>, R_a : seq<bool>)
   } // End else.
 } // End lemma.
 
-lemma BaseCaseRes(a : seq<bool>)
-  ensures Res(a) == ResJoin(Aux_2(a), Res(a), Seen1(a), Aux_2([]), Res([]), Seen1([]))
-  {}
-
 lemma HomRes(a : seq<bool>, R_a : seq<bool>)
   ensures Res(a + R_a) == ResJoin(Aux_2(a), Res(a), Seen1(a), Aux_2(R_a), Res(R_a), Seen1(R_a))
   {
     if R_a == [] 
     {
     assert(a + [] == a);
-    BaseCaseRes(a);
     
      } else {
     calc{
