ocamllibs/dafny_examples/Example_0star1star.dfy
@@ -18,7 +18,7 @@ function Bn(ar : seq<bool>): bool
     true
     else
     (if (! ar[|ar|-1]) then Bn(ar[..|ar|-1]) else
-      (An(ar[..|ar|-1]) && Bn(ar[..|ar|-1])))
+      ((ar[|ar|-1] && An(ar[..|ar|-1])) && Bn(ar[..|ar|-1])))
 }
 
 function Aux_1Join(leftAux_1 : bool, rightAux_1 : bool): bool
@@ -33,7 +33,8 @@ function AnJoin(leftBn : bool, leftAn : bool, rightBn : bool, rightAn : bool): b
 
 function BnJoin(leftAux_1 : bool, leftBn : bool, leftAn : bool, rightAux_1 : bool, rightBn : bool, rightAn : bool): bool
 {
-  (leftAn && rightBn) || ((rightBn && (! rightAux_1) && ((! rightAn) && leftBn)))
+  (if rightAux_1 then (leftAn && rightBn) else
+    ((rightBn || rightAux_1) && ((! rightAn) && leftBn)))
 }
 
 
@@ -46,11 +47,11 @@ lemma HomAux_1(ar : seq<bool>, R_ar : seq<bool>)
   requires |ar| >= 1 && |R_ar| >= 1
   ensures Aux_1(ar + R_ar) == Aux_1Join(Aux_1(ar), Aux_1(R_ar))
   {
-    if |R_ar| == 1
+    if |R_ar| == 1 
     {
     assert(ar + R_ar == ar + [R_ar[0]]);
     BaseCaseAux_1(ar, R_ar);
-
+    
      } else {
     calc{
     Aux_1(ar + R_ar);
@@ -61,12 +62,12 @@ lemma HomAux_1(ar : seq<bool>, R_ar : seq<bool>)
 } // End lemma.
 
 lemma HomAn(ar : seq<bool>, R_ar : seq<bool>)
-	requires |ar| >= 1 && |R_ar| >= 1
   ensures An(ar + R_ar) == AnJoin(Bn(ar), An(ar), Bn(R_ar), An(R_ar))
   {
-    if |R_ar| == 1
+    if R_ar == [] 
     {
-			assert(ar + R_ar == ar + [R_ar[0]]);
+    assert(ar + [] == ar);
+    
      } else {
     calc{
     An(ar + R_ar);
@@ -88,11 +89,11 @@ lemma HomBn(ar : seq<bool>, R_ar : seq<bool>)
   requires |ar| >= 1 && |R_ar| >= 1
   ensures Bn(ar + R_ar) == BnJoin(Aux_1(ar), Bn(ar), An(ar), Aux_1(R_ar), Bn(R_ar), An(R_ar))
   {
-    if |R_ar| == 1
+    if |R_ar| == 1 
     {
     assert(ar + R_ar == ar + [R_ar[0]]);
     BaseCaseBn(ar, R_ar);
-
+    
      } else {
     calc{
     Bn(ar + R_ar);
@@ -105,3 +106,4 @@ lemma HomBn(ar : seq<bool>, R_ar : seq<bool>)
     } // End calc.
   } // End else.
 } // End lemma.
+
